Add a better proof of the fact that closure terminates, this time using a set of available symbols instead of a list

AllStar/Subparser.v
@@ -27,23 +27,102 @@ Definition move (token : string)
       end 
   in  concat (map moveSp sps).
 
+Definition removeOpt (x : symbol) (s : SymbolSet.t) :=
+  if SymbolSet.mem x s then Some (SymbolSet.remove x s) else None.
+
+Lemma empty_nil : forall s,
+    SymbolSet.Empty s <-> SymbolSet.elements s = [].
+Proof. 
+  intros; split; intros.
+  - destruct (SymbolSet.elements s) as [| e es] eqn:Hs.
+    + reflexivity.
+    + exfalso. 
+      unfold SymbolSet.Empty in H; eapply H; clear H.
+      assert (SetoidList.InA eq e (SymbolSet.elements s)).
+      { rewrite Hs; constructor; reflexivity. }
+      eapply SymbolSetFacts.elements_iff. eassumption.
+  - unfold SymbolSet.Empty; unfold not; intros e Hin.
+    rewrite SymbolSetFacts.elements_iff in Hin. 
+    rewrite H in Hin. inv Hin.
+Qed.
+
+Lemma list_remove_le : forall (x : symbol) (ys : list symbol),
+    List.length (remove symbol_eq_dec x ys) <= List.length ys.
+Proof.
+  intros. induction ys as [| y ys]; simpl.
+  - reflexivity.
+  - destruct (symbol_eq_dec x y); simpl; omega.
+Qed.
+
+Lemma list_remove_lt : forall (x : symbol) (ys : list symbol),
+    List.In x ys -> 
+    List.length (remove symbol_eq_dec x ys) < List.length ys.
+Proof.
+  intros. induction ys as [| y ys]; simpl.
+  - inv H.
+  - destruct (symbol_eq_dec x y) as [Heq | Hneq]; simpl.
+    + pose proof list_remove_le as Hle.
+      specialize Hle with (x := x) (ys := ys). omega.
+    + apply lt_n_S. apply IHys. clear IHys.
+      simpl in H. destruct H as [Hhd | Htl].
+      * exfalso. apply Hneq. symmetry. assumption.
+      * assumption.
+Qed.
+
+Lemma cardinal_length : forall s s',
+    SymbolSet.cardinal s' < SymbolSet.cardinal s <-> 
+    List.length (SymbolSet.elements s') < List.length (SymbolSet.elements s).
+Proof.
+  intros. split; intros.
+  - repeat rewrite <- SymbolSet.cardinal_spec. assumption.
+  - repeat rewrite SymbolSet.cardinal_spec. assumption.
+Qed.
+
+Lemma remove_not_In : forall x ys,
+    ~In x ys <-> remove symbol_eq_dec x ys = ys.
+Proof.
+  intros; split; unfold not; intros.
+  - induction ys; simpl.
+    + reflexivity.
+    + destruct (symbol_eq_dec x a); simpl.
+      * exfalso. subst. apply H. apply in_eq.
+      * assert (Htls : remove symbol_eq_dec x ys = ys).
+      { apply IHys; intros; clear IHys.
+        apply H. apply in_cons. assumption. }
+      rewrite Htls; reflexivity.
+  - rewrite <- H in H0. eapply remove_In. eassumption.
+Qed.             
+
+(* HERE is the lemma I needed -- wish I'd found remove_cardinal_1 sooner...*)
+Lemma removeOptDecreasing : forall (x : symbol) (s s' : SymbolSet.t),
+    removeOpt x s = Some s' ->
+    SymbolSet.cardinal s' < SymbolSet.cardinal s.
+Proof.
+  intros. unfold removeOpt in H. 
+  destruct (SymbolSet.mem x s) eqn:Hmem.
+  - inv H.
+    pose proof SymbolSetEqProps.remove_cardinal_1.
+    apply H in Hmem. omega.
+  - inv H.
+Qed.
+
 (* if removeOpt x l  = Some l', l' is a sublist of l *)
-Fixpoint removeOpt {A} (x : A) (l : list A) (beq : A -> A -> bool) :=
+Fixpoint removeOpt' {A} (x : A) (l : list A) (beq : A -> A -> bool) :=
   match l with
   | nil => None
   | y :: l' => 
     if beq x y then
       Some l'
     else
-      match removeOpt x l' beq with
+      match removeOpt' x l' beq with
       | None => None
       | Some l'' => Some (y :: l'')
       end
   end.
 
 (* ... and here's the proof: *)
-Lemma removeOptDecreasing : forall A (x : A) beq (ys zs : list A),
-    removeOpt x ys beq = Some zs ->
+Lemma removeOpt'Decreasing : forall A (x : A) beq (ys zs : list A),
+    removeOpt' x ys beq = Some zs ->
     List.length zs < List.length ys.
 Proof.
   induction ys as [| y ys]; intros zs H.
@@ -51,30 +130,10 @@ Proof.
   - simpl in H.
     destruct (beq x y).
     + inv H; simpl; omega.
-    + destruct (removeOpt x ys beq).
+    + destruct (removeOpt' x ys beq).
       * inv H. simpl.
         apply lt_n_S; apply IHys; reflexivity.
       * inv H.
-Qed.
-
-(* Here's a better way to handle removing elements from the free set. *)
-
-Definition removeOpt' (x : symbol) (s : SymbolSet.t) :=
-  let s' := SymbolSet.remove x s in
-  if (SymbolSet.cardinal s') <? (SymbolSet.cardinal s) then
-    Some s'
-  else
-    None.
-
-Lemma removeOpt'Decreasing : forall (x : symbol) (ys zs : SymbolSet.t),
-    removeOpt' x ys = Some zs ->
-    SymbolSet.cardinal zs < SymbolSet.cardinal ys.
-Proof.
-  intros. unfold removeOpt' in H.
-  destruct (SymbolSet.cardinal (SymbolSet.remove x ys) <? SymbolSet.cardinal ys)
-           eqn:Heq.
-  - inv H. rewrite <- Nat.ltb_lt. assumption.
-  - inv H.
 Qed.
 
 Program Fixpoint spClosure (g : grammar)
@@ -86,7 +145,7 @@ Program Fixpoint spClosure (g : grammar)
        | nil => [sp]
        | T _ :: _ => [sp]
        | NT x :: stack' => 
-         match removeOpt (NT x) freeSyms beqSym with
+         match removeOpt' (NT x) freeSyms beqSym with
          | None => nil (* recursion detected *)
          | Some freeSyms' => 
            concat (map (fun gamma => 
@@ -95,7 +154,7 @@ Program Fixpoint spClosure (g : grammar)
          end
        end.
 Obligation 1.
-eapply removeOptDecreasing. symmetry. eassumption.
+eapply removeOpt'Decreasing. symmetry. eassumption.
 Qed.
 
 Definition nonterminals g :=
