Lib/Grammar.v
@@ -29,6 +29,7 @@ Module SymbolAsDT := Make_UDT(MDT_Symbol).
 
 Module SymbolSet := MSetWeakList.Make SymbolAsDT.
 Module SymbolSetFacts := WFactsOn SymbolAsDT SymbolSet.
+Module SymbolSetEqProps := EqProperties SymbolSet.
 
 Module SymbolMap := FMapWeakList.Make SymbolAsDT.
 Module SymbolMapFacts := WFacts_fun SymbolAsDT SymbolMap.
